Traces.v
@@ -10,4 +10,47 @@ Infix "::" := Tcons (at level 60, right associativity) : trace_scope.
 Notation "[ ]" := Tnil (format "[ ]") : trace_scope.
 Notation "[ x ]" := (Tcons Tnil x) : trace_scope.
 Notation "[ x ; .. ; y ; z ]" := (Tcons (Tcons .. (Tcons Tnil x) .. y) z)
-  (format "[ '[' x ; '/' .. ; '/' y ; '/' z ']' ]") : list_scope.
+  (format "[ '[' x ; '/' .. ; '/' y ; '/' z ']' ]") : trace_scope.
+
+Open Scope trace_scope.
+
+Fixpoint app {A:Type} (xs ys:trace A) : trace A :=
+  match ys with
+  | [] => xs
+  | ys :: y => (app xs ys) :: y
+  end.
+
+Notation "x '++' y" := (app x y) : trace_scope.
+
+Theorem app_nil_l {A:Type} (x:trace A) : [] ++ x = x.
+Proof. induction x. reflexivity. simpl. rewrite IHx. reflexivity. Qed.
+
+Theorem app_nil_r {A:Type} (x:trace A) : x ++ [] = x.
+Proof. reflexivity. Qed.
+
+Theorem app_comm_cons {A:Type} (a:A) (x y:trace A) : (x ++ y) :: a = x ++ (y :: a).
+Proof. reflexivity. Qed.
+
+Theorem app_assoc {A:Type} (x y z:trace A) : x ++ y ++ z = (x ++ y) ++ z.
+Proof.
+  induction z.
+  - reflexivity.
+  - simpl. rewrite IHz. reflexivity.
+Qed.
+
+Lemma cons_not_empty {A:Type} (a:A) (t:trace A) : t :: a <> [].
+Proof.
+  intros. induction t.
+  - discriminate.
+  - discriminate.
+Qed.
+
+Theorem app_eq_nil {A:Type} (x y:trace A) : x ++ y = [] -> x = [] /\ y = [].
+Proof.
+  induction y; induction x; intro; split;
+    try (rewrite app_nil_r in H);
+    try (rewrite app_nil_l in H);
+    try reflexivity;
+    try assumption;
+    discriminate.
+Qed.
